AwsCryptographicMaterialProviders/runtimes/net/Generated/AwsCryptographyKeyStore/NativeWrapper_KeyStorageInterface.cs
@@ -17,62 +17,6 @@ namespace AWS.Cryptography.KeyStore
     {
       _impl = nativeImpl;
     }
-    public Wrappers_Compile._IResult<software.amazon.cryptography.keystore.internaldafny.types._IGetEncryptedActiveBranchKeyOutput, software.amazon.cryptography.keystore.internaldafny.types._IError> GetEncryptedActiveBranchKey(software.amazon.cryptography.keystore.internaldafny.types._IGetEncryptedActiveBranchKeyInput input)
-    {
-      void validateOutput(AWS.Cryptography.KeyStore.GetEncryptedActiveBranchKeyOutput nativeOutput)
-      {
-        try { nativeOutput.Validate(); }
-        catch (ArgumentException e)
-        {
-          var message = $"Output of {_impl}._GetEncryptedActiveBranchKey is invalid. {e.Message}";
-          throw new KeyStoreException(message);
-        }
-      }
-      AWS.Cryptography.KeyStore.GetEncryptedActiveBranchKeyInput nativeInput = TypeConversion.FromDafny_N3_aws__N12_cryptography__N8_keyStore__S32_GetEncryptedActiveBranchKeyInput(input);
-      try
-      {
-        AWS.Cryptography.KeyStore.GetEncryptedActiveBranchKeyOutput nativeOutput = _impl.GetEncryptedActiveBranchKey(nativeInput);
-        _ = nativeOutput ?? throw new KeyStoreException($"{_impl}._GetEncryptedActiveBranchKey returned null, should be {typeof(AWS.Cryptography.KeyStore.GetEncryptedActiveBranchKeyOutput)}");
-        validateOutput(nativeOutput);
-        return Wrappers_Compile.Result<software.amazon.cryptography.keystore.internaldafny.types._IGetEncryptedActiveBranchKeyOutput, software.amazon.cryptography.keystore.internaldafny.types._IError>.create_Success(TypeConversion.ToDafny_N3_aws__N12_cryptography__N8_keyStore__S33_GetEncryptedActiveBranchKeyOutput(nativeOutput));
-      }
-      catch (Exception e)
-      {
-        return Wrappers_Compile.Result<software.amazon.cryptography.keystore.internaldafny.types._IGetEncryptedActiveBranchKeyOutput, software.amazon.cryptography.keystore.internaldafny.types._IError>.create_Failure(TypeConversion.ToDafny_CommonError(e));
-      }
-    }
-    public Wrappers_Compile._IResult<software.amazon.cryptography.keystore.internaldafny.types._IGetEncryptedActiveBranchKeyOutput, software.amazon.cryptography.keystore.internaldafny.types._IError> GetEncryptedActiveBranchKey_k(software.amazon.cryptography.keystore.internaldafny.types._IGetEncryptedActiveBranchKeyInput input)
-    {
-      throw new KeyStoreException("Not supported at this time.");
-    }
-    public Wrappers_Compile._IResult<software.amazon.cryptography.keystore.internaldafny.types._IWriteMutatedVersionsOutput, software.amazon.cryptography.keystore.internaldafny.types._IError> WriteMutatedVersions(software.amazon.cryptography.keystore.internaldafny.types._IWriteMutatedVersionsInput input)
-    {
-      void validateOutput(AWS.Cryptography.KeyStore.WriteMutatedVersionsOutput nativeOutput)
-      {
-        try { nativeOutput.Validate(); }
-        catch (ArgumentException e)
-        {
-          var message = $"Output of {_impl}._WriteMutatedVersions is invalid. {e.Message}";
-          throw new KeyStoreException(message);
-        }
-      }
-      AWS.Cryptography.KeyStore.WriteMutatedVersionsInput nativeInput = TypeConversion.FromDafny_N3_aws__N12_cryptography__N8_keyStore__S25_WriteMutatedVersionsInput(input);
-      try
-      {
-        AWS.Cryptography.KeyStore.WriteMutatedVersionsOutput nativeOutput = _impl.WriteMutatedVersions(nativeInput);
-        _ = nativeOutput ?? throw new KeyStoreException($"{_impl}._WriteMutatedVersions returned null, should be {typeof(AWS.Cryptography.KeyStore.WriteMutatedVersionsOutput)}");
-        validateOutput(nativeOutput);
-        return Wrappers_Compile.Result<software.amazon.cryptography.keystore.internaldafny.types._IWriteMutatedVersionsOutput, software.amazon.cryptography.keystore.internaldafny.types._IError>.create_Success(TypeConversion.ToDafny_N3_aws__N12_cryptography__N8_keyStore__S26_WriteMutatedVersionsOutput(nativeOutput));
-      }
-      catch (Exception e)
-      {
-        return Wrappers_Compile.Result<software.amazon.cryptography.keystore.internaldafny.types._IWriteMutatedVersionsOutput, software.amazon.cryptography.keystore.internaldafny.types._IError>.create_Failure(TypeConversion.ToDafny_CommonError(e));
-      }
-    }
-    public Wrappers_Compile._IResult<software.amazon.cryptography.keystore.internaldafny.types._IWriteMutatedVersionsOutput, software.amazon.cryptography.keystore.internaldafny.types._IError> WriteMutatedVersions_k(software.amazon.cryptography.keystore.internaldafny.types._IWriteMutatedVersionsInput input)
-    {
-      throw new KeyStoreException("Not supported at this time.");
-    }
     public Wrappers_Compile._IResult<software.amazon.cryptography.keystore.internaldafny.types._IWriteNewEncryptedBranchKeyOutput, software.amazon.cryptography.keystore.internaldafny.types._IError> WriteNewEncryptedBranchKey(software.amazon.cryptography.keystore.internaldafny.types._IWriteNewEncryptedBranchKeyInput input)
     {
       void validateOutput(AWS.Cryptography.KeyStore.WriteNewEncryptedBranchKeyOutput nativeOutput)
@@ -98,62 +42,6 @@ namespace AWS.Cryptography.KeyStore
       }
     }
     public Wrappers_Compile._IResult<software.amazon.cryptography.keystore.internaldafny.types._IWriteNewEncryptedBranchKeyOutput, software.amazon.cryptography.keystore.internaldafny.types._IError> WriteNewEncryptedBranchKey_k(software.amazon.cryptography.keystore.internaldafny.types._IWriteNewEncryptedBranchKeyInput input)
-    {
-      throw new KeyStoreException("Not supported at this time.");
-    }
-    public Wrappers_Compile._IResult<software.amazon.cryptography.keystore.internaldafny.types._IWriteInitializeMutationOutput, software.amazon.cryptography.keystore.internaldafny.types._IError> WriteInitializeMutation(software.amazon.cryptography.keystore.internaldafny.types._IWriteInitializeMutationInput input)
-    {
-      void validateOutput(AWS.Cryptography.KeyStore.WriteInitializeMutationOutput nativeOutput)
-      {
-        try { nativeOutput.Validate(); }
-        catch (ArgumentException e)
-        {
-          var message = $"Output of {_impl}._WriteInitializeMutation is invalid. {e.Message}";
-          throw new KeyStoreException(message);
-        }
-      }
-      AWS.Cryptography.KeyStore.WriteInitializeMutationInput nativeInput = TypeConversion.FromDafny_N3_aws__N12_cryptography__N8_keyStore__S28_WriteInitializeMutationInput(input);
-      try
-      {
-        AWS.Cryptography.KeyStore.WriteInitializeMutationOutput nativeOutput = _impl.WriteInitializeMutation(nativeInput);
-        _ = nativeOutput ?? throw new KeyStoreException($"{_impl}._WriteInitializeMutation returned null, should be {typeof(AWS.Cryptography.KeyStore.WriteInitializeMutationOutput)}");
-        validateOutput(nativeOutput);
-        return Wrappers_Compile.Result<software.amazon.cryptography.keystore.internaldafny.types._IWriteInitializeMutationOutput, software.amazon.cryptography.keystore.internaldafny.types._IError>.create_Success(TypeConversion.ToDafny_N3_aws__N12_cryptography__N8_keyStore__S29_WriteInitializeMutationOutput(nativeOutput));
-      }
-      catch (Exception e)
-      {
-        return Wrappers_Compile.Result<software.amazon.cryptography.keystore.internaldafny.types._IWriteInitializeMutationOutput, software.amazon.cryptography.keystore.internaldafny.types._IError>.create_Failure(TypeConversion.ToDafny_CommonError(e));
-      }
-    }
-    public Wrappers_Compile._IResult<software.amazon.cryptography.keystore.internaldafny.types._IWriteInitializeMutationOutput, software.amazon.cryptography.keystore.internaldafny.types._IError> WriteInitializeMutation_k(software.amazon.cryptography.keystore.internaldafny.types._IWriteInitializeMutationInput input)
-    {
-      throw new KeyStoreException("Not supported at this time.");
-    }
-    public Wrappers_Compile._IResult<software.amazon.cryptography.keystore.internaldafny.types._IGetMutationOutput, software.amazon.cryptography.keystore.internaldafny.types._IError> GetMutation(software.amazon.cryptography.keystore.internaldafny.types._IGetMutationInput input)
-    {
-      void validateOutput(AWS.Cryptography.KeyStore.GetMutationOutput nativeOutput)
-      {
-        try { nativeOutput.Validate(); }
-        catch (ArgumentException e)
-        {
-          var message = $"Output of {_impl}._GetMutation is invalid. {e.Message}";
-          throw new KeyStoreException(message);
-        }
-      }
-      AWS.Cryptography.KeyStore.GetMutationInput nativeInput = TypeConversion.FromDafny_N3_aws__N12_cryptography__N8_keyStore__S16_GetMutationInput(input);
-      try
-      {
-        AWS.Cryptography.KeyStore.GetMutationOutput nativeOutput = _impl.GetMutation(nativeInput);
-        _ = nativeOutput ?? throw new KeyStoreException($"{_impl}._GetMutation returned null, should be {typeof(AWS.Cryptography.KeyStore.GetMutationOutput)}");
-        validateOutput(nativeOutput);
-        return Wrappers_Compile.Result<software.amazon.cryptography.keystore.internaldafny.types._IGetMutationOutput, software.amazon.cryptography.keystore.internaldafny.types._IError>.create_Success(TypeConversion.ToDafny_N3_aws__N12_cryptography__N8_keyStore__S17_GetMutationOutput(nativeOutput));
-      }
-      catch (Exception e)
-      {
-        return Wrappers_Compile.Result<software.amazon.cryptography.keystore.internaldafny.types._IGetMutationOutput, software.amazon.cryptography.keystore.internaldafny.types._IError>.create_Failure(TypeConversion.ToDafny_CommonError(e));
-      }
-    }
-    public Wrappers_Compile._IResult<software.amazon.cryptography.keystore.internaldafny.types._IGetMutationOutput, software.amazon.cryptography.keystore.internaldafny.types._IError> GetMutation_k(software.amazon.cryptography.keystore.internaldafny.types._IGetMutationInput input)
     {
       throw new KeyStoreException("Not supported at this time.");
     }
@@ -185,59 +73,31 @@ namespace AWS.Cryptography.KeyStore
     {
       throw new KeyStoreException("Not supported at this time.");
     }
-    public Wrappers_Compile._IResult<software.amazon.cryptography.keystore.internaldafny.types._IWriteNewEncryptedBranchKeyVersionOutput, software.amazon.cryptography.keystore.internaldafny.types._IError> WriteNewEncryptedBranchKeyVersion(software.amazon.cryptography.keystore.internaldafny.types._IWriteNewEncryptedBranchKeyVersionInput input)
+    public Wrappers_Compile._IResult<software.amazon.cryptography.keystore.internaldafny.types._IGetMutationLockOutput, software.amazon.cryptography.keystore.internaldafny.types._IError> GetMutationLock(software.amazon.cryptography.keystore.internaldafny.types._IGetMutationLockInput input)
     {
-      void validateOutput(AWS.Cryptography.KeyStore.WriteNewEncryptedBranchKeyVersionOutput nativeOutput)
+      void validateOutput(AWS.Cryptography.KeyStore.GetMutationLockOutput nativeOutput)
       {
         try { nativeOutput.Validate(); }
         catch (ArgumentException e)
         {
-          var message = $"Output of {_impl}._WriteNewEncryptedBranchKeyVersion is invalid. {e.Message}";
+          var message = $"Output of {_impl}._GetMutationLock is invalid. {e.Message}";
           throw new KeyStoreException(message);
         }
       }
-      AWS.Cryptography.KeyStore.WriteNewEncryptedBranchKeyVersionInput nativeInput = TypeConversion.FromDafny_N3_aws__N12_cryptography__N8_keyStore__S38_WriteNewEncryptedBranchKeyVersionInput(input);
+      AWS.Cryptography.KeyStore.GetMutationLockInput nativeInput = TypeConversion.FromDafny_N3_aws__N12_cryptography__N8_keyStore__S20_GetMutationLockInput(input);
       try
       {
-        AWS.Cryptography.KeyStore.WriteNewEncryptedBranchKeyVersionOutput nativeOutput = _impl.WriteNewEncryptedBranchKeyVersion(nativeInput);
-        _ = nativeOutput ?? throw new KeyStoreException($"{_impl}._WriteNewEncryptedBranchKeyVersion returned null, should be {typeof(AWS.Cryptography.KeyStore.WriteNewEncryptedBranchKeyVersionOutput)}");
+        AWS.Cryptography.KeyStore.GetMutationLockOutput nativeOutput = _impl.GetMutationLock(nativeInput);
+        _ = nativeOutput ?? throw new KeyStoreException($"{_impl}._GetMutationLock returned null, should be {typeof(AWS.Cryptography.KeyStore.GetMutationLockOutput)}");
         validateOutput(nativeOutput);
-        return Wrappers_Compile.Result<software.amazon.cryptography.keystore.internaldafny.types._IWriteNewEncryptedBranchKeyVersionOutput, software.amazon.cryptography.keystore.internaldafny.types._IError>.create_Success(TypeConversion.ToDafny_N3_aws__N12_cryptography__N8_keyStore__S39_WriteNewEncryptedBranchKeyVersionOutput(nativeOutput));
+        return Wrappers_Compile.Result<software.amazon.cryptography.keystore.internaldafny.types._IGetMutationLockOutput, software.amazon.cryptography.keystore.internaldafny.types._IError>.create_Success(TypeConversion.ToDafny_N3_aws__N12_cryptography__N8_keyStore__S21_GetMutationLockOutput(nativeOutput));
       }
       catch (Exception e)
       {
-        return Wrappers_Compile.Result<software.amazon.cryptography.keystore.internaldafny.types._IWriteNewEncryptedBranchKeyVersionOutput, software.amazon.cryptography.keystore.internaldafny.types._IError>.create_Failure(TypeConversion.ToDafny_CommonError(e));
+        return Wrappers_Compile.Result<software.amazon.cryptography.keystore.internaldafny.types._IGetMutationLockOutput, software.amazon.cryptography.keystore.internaldafny.types._IError>.create_Failure(TypeConversion.ToDafny_CommonError(e));
       }
     }
-    public Wrappers_Compile._IResult<software.amazon.cryptography.keystore.internaldafny.types._IWriteNewEncryptedBranchKeyVersionOutput, software.amazon.cryptography.keystore.internaldafny.types._IError> WriteNewEncryptedBranchKeyVersion_k(software.amazon.cryptography.keystore.internaldafny.types._IWriteNewEncryptedBranchKeyVersionInput input)
-    {
-      throw new KeyStoreException("Not supported at this time.");
-    }
-    public Wrappers_Compile._IResult<software.amazon.cryptography.keystore.internaldafny.types._IQueryForVersionsOutput, software.amazon.cryptography.keystore.internaldafny.types._IError> QueryForVersions(software.amazon.cryptography.keystore.internaldafny.types._IQueryForVersionsInput input)
-    {
-      void validateOutput(AWS.Cryptography.KeyStore.QueryForVersionsOutput nativeOutput)
-      {
-        try { nativeOutput.Validate(); }
-        catch (ArgumentException e)
-        {
-          var message = $"Output of {_impl}._QueryForVersions is invalid. {e.Message}";
-          throw new KeyStoreException(message);
-        }
-      }
-      AWS.Cryptography.KeyStore.QueryForVersionsInput nativeInput = TypeConversion.FromDafny_N3_aws__N12_cryptography__N8_keyStore__S21_QueryForVersionsInput(input);
-      try
-      {
-        AWS.Cryptography.KeyStore.QueryForVersionsOutput nativeOutput = _impl.QueryForVersions(nativeInput);
-        _ = nativeOutput ?? throw new KeyStoreException($"{_impl}._QueryForVersions returned null, should be {typeof(AWS.Cryptography.KeyStore.QueryForVersionsOutput)}");
-        validateOutput(nativeOutput);
-        return Wrappers_Compile.Result<software.amazon.cryptography.keystore.internaldafny.types._IQueryForVersionsOutput, software.amazon.cryptography.keystore.internaldafny.types._IError>.create_Success(TypeConversion.ToDafny_N3_aws__N12_cryptography__N8_keyStore__S22_QueryForVersionsOutput(nativeOutput));
-      }
-      catch (Exception e)
-      {
-        return Wrappers_Compile.Result<software.amazon.cryptography.keystore.internaldafny.types._IQueryForVersionsOutput, software.amazon.cryptography.keystore.internaldafny.types._IError>.create_Failure(TypeConversion.ToDafny_CommonError(e));
-      }
-    }
-    public Wrappers_Compile._IResult<software.amazon.cryptography.keystore.internaldafny.types._IQueryForVersionsOutput, software.amazon.cryptography.keystore.internaldafny.types._IError> QueryForVersions_k(software.amazon.cryptography.keystore.internaldafny.types._IQueryForVersionsInput input)
+    public Wrappers_Compile._IResult<software.amazon.cryptography.keystore.internaldafny.types._IGetMutationLockOutput, software.amazon.cryptography.keystore.internaldafny.types._IError> GetMutationLock_k(software.amazon.cryptography.keystore.internaldafny.types._IGetMutationLockInput input)
     {
       throw new KeyStoreException("Not supported at this time.");
     }
@@ -297,31 +157,31 @@ namespace AWS.Cryptography.KeyStore
     {
       throw new KeyStoreException("Not supported at this time.");
     }
-    public Wrappers_Compile._IResult<software.amazon.cryptography.keystore.internaldafny.types._IDeleteMutationOutput, software.amazon.cryptography.keystore.internaldafny.types._IError> DeleteMutation(software.amazon.cryptography.keystore.internaldafny.types._IDeleteMutationInput input)
+    public Wrappers_Compile._IResult<software.amazon.cryptography.keystore.internaldafny.types._IDeleteMutationLockAndIndexOutput, software.amazon.cryptography.keystore.internaldafny.types._IError> DeleteMutationLockAndIndex(software.amazon.cryptography.keystore.internaldafny.types._IDeleteMutationLockAndIndexInput input)
     {
-      void validateOutput(AWS.Cryptography.KeyStore.DeleteMutationOutput nativeOutput)
+      void validateOutput(AWS.Cryptography.KeyStore.DeleteMutationLockAndIndexOutput nativeOutput)
       {
         try { nativeOutput.Validate(); }
         catch (ArgumentException e)
         {
-          var message = $"Output of {_impl}._DeleteMutation is invalid. {e.Message}";
+          var message = $"Output of {_impl}._DeleteMutationLockAndIndex is invalid. {e.Message}";
           throw new KeyStoreException(message);
         }
       }
-      AWS.Cryptography.KeyStore.DeleteMutationInput nativeInput = TypeConversion.FromDafny_N3_aws__N12_cryptography__N8_keyStore__S19_DeleteMutationInput(input);
+      AWS.Cryptography.KeyStore.DeleteMutationLockAndIndexInput nativeInput = TypeConversion.FromDafny_N3_aws__N12_cryptography__N8_keyStore__S31_DeleteMutationLockAndIndexInput(input);
       try
       {
-        AWS.Cryptography.KeyStore.DeleteMutationOutput nativeOutput = _impl.DeleteMutation(nativeInput);
-        _ = nativeOutput ?? throw new KeyStoreException($"{_impl}._DeleteMutation returned null, should be {typeof(AWS.Cryptography.KeyStore.DeleteMutationOutput)}");
+        AWS.Cryptography.KeyStore.DeleteMutationLockAndIndexOutput nativeOutput = _impl.DeleteMutationLockAndIndex(nativeInput);
+        _ = nativeOutput ?? throw new KeyStoreException($"{_impl}._DeleteMutationLockAndIndex returned null, should be {typeof(AWS.Cryptography.KeyStore.DeleteMutationLockAndIndexOutput)}");
         validateOutput(nativeOutput);
-        return Wrappers_Compile.Result<software.amazon.cryptography.keystore.internaldafny.types._IDeleteMutationOutput, software.amazon.cryptography.keystore.internaldafny.types._IError>.create_Success(TypeConversion.ToDafny_N3_aws__N12_cryptography__N8_keyStore__S20_DeleteMutationOutput(nativeOutput));
+        return Wrappers_Compile.Result<software.amazon.cryptography.keystore.internaldafny.types._IDeleteMutationLockAndIndexOutput, software.amazon.cryptography.keystore.internaldafny.types._IError>.create_Success(TypeConversion.ToDafny_N3_aws__N12_cryptography__N8_keyStore__S32_DeleteMutationLockAndIndexOutput(nativeOutput));
       }
       catch (Exception e)
       {
-        return Wrappers_Compile.Result<software.amazon.cryptography.keystore.internaldafny.types._IDeleteMutationOutput, software.amazon.cryptography.keystore.internaldafny.types._IError>.create_Failure(TypeConversion.ToDafny_CommonError(e));
+        return Wrappers_Compile.Result<software.amazon.cryptography.keystore.internaldafny.types._IDeleteMutationLockAndIndexOutput, software.amazon.cryptography.keystore.internaldafny.types._IError>.create_Failure(TypeConversion.ToDafny_CommonError(e));
       }
     }
-    public Wrappers_Compile._IResult<software.amazon.cryptography.keystore.internaldafny.types._IDeleteMutationOutput, software.amazon.cryptography.keystore.internaldafny.types._IError> DeleteMutation_k(software.amazon.cryptography.keystore.internaldafny.types._IDeleteMutationInput input)
+    public Wrappers_Compile._IResult<software.amazon.cryptography.keystore.internaldafny.types._IDeleteMutationLockAndIndexOutput, software.amazon.cryptography.keystore.internaldafny.types._IError> DeleteMutationLockAndIndex_k(software.amazon.cryptography.keystore.internaldafny.types._IDeleteMutationLockAndIndexInput input)
     {
       throw new KeyStoreException("Not supported at this time.");
     }
@@ -350,6 +210,202 @@ namespace AWS.Cryptography.KeyStore
       }
     }
     public Wrappers_Compile._IResult<software.amazon.cryptography.keystore.internaldafny.types._IGetEncryptedBeaconKeyOutput, software.amazon.cryptography.keystore.internaldafny.types._IError> GetEncryptedBeaconKey_k(software.amazon.cryptography.keystore.internaldafny.types._IGetEncryptedBeaconKeyInput input)
+    {
+      throw new KeyStoreException("Not supported at this time.");
+    }
+    public Wrappers_Compile._IResult<software.amazon.cryptography.keystore.internaldafny.types._IGetEncryptedActiveBranchKeyOutput, software.amazon.cryptography.keystore.internaldafny.types._IError> GetEncryptedActiveBranchKey(software.amazon.cryptography.keystore.internaldafny.types._IGetEncryptedActiveBranchKeyInput input)
+    {
+      void validateOutput(AWS.Cryptography.KeyStore.GetEncryptedActiveBranchKeyOutput nativeOutput)
+      {
+        try { nativeOutput.Validate(); }
+        catch (ArgumentException e)
+        {
+          var message = $"Output of {_impl}._GetEncryptedActiveBranchKey is invalid. {e.Message}";
+          throw new KeyStoreException(message);
+        }
+      }
+      AWS.Cryptography.KeyStore.GetEncryptedActiveBranchKeyInput nativeInput = TypeConversion.FromDafny_N3_aws__N12_cryptography__N8_keyStore__S32_GetEncryptedActiveBranchKeyInput(input);
+      try
+      {
+        AWS.Cryptography.KeyStore.GetEncryptedActiveBranchKeyOutput nativeOutput = _impl.GetEncryptedActiveBranchKey(nativeInput);
+        _ = nativeOutput ?? throw new KeyStoreException($"{_impl}._GetEncryptedActiveBranchKey returned null, should be {typeof(AWS.Cryptography.KeyStore.GetEncryptedActiveBranchKeyOutput)}");
+        validateOutput(nativeOutput);
+        return Wrappers_Compile.Result<software.amazon.cryptography.keystore.internaldafny.types._IGetEncryptedActiveBranchKeyOutput, software.amazon.cryptography.keystore.internaldafny.types._IError>.create_Success(TypeConversion.ToDafny_N3_aws__N12_cryptography__N8_keyStore__S33_GetEncryptedActiveBranchKeyOutput(nativeOutput));
+      }
+      catch (Exception e)
+      {
+        return Wrappers_Compile.Result<software.amazon.cryptography.keystore.internaldafny.types._IGetEncryptedActiveBranchKeyOutput, software.amazon.cryptography.keystore.internaldafny.types._IError>.create_Failure(TypeConversion.ToDafny_CommonError(e));
+      }
+    }
+    public Wrappers_Compile._IResult<software.amazon.cryptography.keystore.internaldafny.types._IGetEncryptedActiveBranchKeyOutput, software.amazon.cryptography.keystore.internaldafny.types._IError> GetEncryptedActiveBranchKey_k(software.amazon.cryptography.keystore.internaldafny.types._IGetEncryptedActiveBranchKeyInput input)
+    {
+      throw new KeyStoreException("Not supported at this time.");
+    }
+    public Wrappers_Compile._IResult<software.amazon.cryptography.keystore.internaldafny.types._IWriteMutatedVersionsOutput, software.amazon.cryptography.keystore.internaldafny.types._IError> WriteMutatedVersions(software.amazon.cryptography.keystore.internaldafny.types._IWriteMutatedVersionsInput input)
+    {
+      void validateOutput(AWS.Cryptography.KeyStore.WriteMutatedVersionsOutput nativeOutput)
+      {
+        try { nativeOutput.Validate(); }
+        catch (ArgumentException e)
+        {
+          var message = $"Output of {_impl}._WriteMutatedVersions is invalid. {e.Message}";
+          throw new KeyStoreException(message);
+        }
+      }
+      AWS.Cryptography.KeyStore.WriteMutatedVersionsInput nativeInput = TypeConversion.FromDafny_N3_aws__N12_cryptography__N8_keyStore__S25_WriteMutatedVersionsInput(input);
+      try
+      {
+        AWS.Cryptography.KeyStore.WriteMutatedVersionsOutput nativeOutput = _impl.WriteMutatedVersions(nativeInput);
+        _ = nativeOutput ?? throw new KeyStoreException($"{_impl}._WriteMutatedVersions returned null, should be {typeof(AWS.Cryptography.KeyStore.WriteMutatedVersionsOutput)}");
+        validateOutput(nativeOutput);
+        return Wrappers_Compile.Result<software.amazon.cryptography.keystore.internaldafny.types._IWriteMutatedVersionsOutput, software.amazon.cryptography.keystore.internaldafny.types._IError>.create_Success(TypeConversion.ToDafny_N3_aws__N12_cryptography__N8_keyStore__S26_WriteMutatedVersionsOutput(nativeOutput));
+      }
+      catch (Exception e)
+      {
+        return Wrappers_Compile.Result<software.amazon.cryptography.keystore.internaldafny.types._IWriteMutatedVersionsOutput, software.amazon.cryptography.keystore.internaldafny.types._IError>.create_Failure(TypeConversion.ToDafny_CommonError(e));
+      }
+    }
+    public Wrappers_Compile._IResult<software.amazon.cryptography.keystore.internaldafny.types._IWriteMutatedVersionsOutput, software.amazon.cryptography.keystore.internaldafny.types._IError> WriteMutatedVersions_k(software.amazon.cryptography.keystore.internaldafny.types._IWriteMutatedVersionsInput input)
+    {
+      throw new KeyStoreException("Not supported at this time.");
+    }
+    public Wrappers_Compile._IResult<software.amazon.cryptography.keystore.internaldafny.types._IWriteInitializeMutationOutput, software.amazon.cryptography.keystore.internaldafny.types._IError> WriteInitializeMutation(software.amazon.cryptography.keystore.internaldafny.types._IWriteInitializeMutationInput input)
+    {
+      void validateOutput(AWS.Cryptography.KeyStore.WriteInitializeMutationOutput nativeOutput)
+      {
+        try { nativeOutput.Validate(); }
+        catch (ArgumentException e)
+        {
+          var message = $"Output of {_impl}._WriteInitializeMutation is invalid. {e.Message}";
+          throw new KeyStoreException(message);
+        }
+      }
+      AWS.Cryptography.KeyStore.WriteInitializeMutationInput nativeInput = TypeConversion.FromDafny_N3_aws__N12_cryptography__N8_keyStore__S28_WriteInitializeMutationInput(input);
+      try
+      {
+        AWS.Cryptography.KeyStore.WriteInitializeMutationOutput nativeOutput = _impl.WriteInitializeMutation(nativeInput);
+        _ = nativeOutput ?? throw new KeyStoreException($"{_impl}._WriteInitializeMutation returned null, should be {typeof(AWS.Cryptography.KeyStore.WriteInitializeMutationOutput)}");
+        validateOutput(nativeOutput);
+        return Wrappers_Compile.Result<software.amazon.cryptography.keystore.internaldafny.types._IWriteInitializeMutationOutput, software.amazon.cryptography.keystore.internaldafny.types._IError>.create_Success(TypeConversion.ToDafny_N3_aws__N12_cryptography__N8_keyStore__S29_WriteInitializeMutationOutput(nativeOutput));
+      }
+      catch (Exception e)
+      {
+        return Wrappers_Compile.Result<software.amazon.cryptography.keystore.internaldafny.types._IWriteInitializeMutationOutput, software.amazon.cryptography.keystore.internaldafny.types._IError>.create_Failure(TypeConversion.ToDafny_CommonError(e));
+      }
+    }
+    public Wrappers_Compile._IResult<software.amazon.cryptography.keystore.internaldafny.types._IWriteInitializeMutationOutput, software.amazon.cryptography.keystore.internaldafny.types._IError> WriteInitializeMutation_k(software.amazon.cryptography.keystore.internaldafny.types._IWriteInitializeMutationInput input)
+    {
+      throw new KeyStoreException("Not supported at this time.");
+    }
+    public Wrappers_Compile._IResult<software.amazon.cryptography.keystore.internaldafny.types._IWriteNewEncryptedBranchKeyVersionOutput, software.amazon.cryptography.keystore.internaldafny.types._IError> WriteNewEncryptedBranchKeyVersion(software.amazon.cryptography.keystore.internaldafny.types._IWriteNewEncryptedBranchKeyVersionInput input)
+    {
+      void validateOutput(AWS.Cryptography.KeyStore.WriteNewEncryptedBranchKeyVersionOutput nativeOutput)
+      {
+        try { nativeOutput.Validate(); }
+        catch (ArgumentException e)
+        {
+          var message = $"Output of {_impl}._WriteNewEncryptedBranchKeyVersion is invalid. {e.Message}";
+          throw new KeyStoreException(message);
+        }
+      }
+      AWS.Cryptography.KeyStore.WriteNewEncryptedBranchKeyVersionInput nativeInput = TypeConversion.FromDafny_N3_aws__N12_cryptography__N8_keyStore__S38_WriteNewEncryptedBranchKeyVersionInput(input);
+      try
+      {
+        AWS.Cryptography.KeyStore.WriteNewEncryptedBranchKeyVersionOutput nativeOutput = _impl.WriteNewEncryptedBranchKeyVersion(nativeInput);
+        _ = nativeOutput ?? throw new KeyStoreException($"{_impl}._WriteNewEncryptedBranchKeyVersion returned null, should be {typeof(AWS.Cryptography.KeyStore.WriteNewEncryptedBranchKeyVersionOutput)}");
+        validateOutput(nativeOutput);
+        return Wrappers_Compile.Result<software.amazon.cryptography.keystore.internaldafny.types._IWriteNewEncryptedBranchKeyVersionOutput, software.amazon.cryptography.keystore.internaldafny.types._IError>.create_Success(TypeConversion.ToDafny_N3_aws__N12_cryptography__N8_keyStore__S39_WriteNewEncryptedBranchKeyVersionOutput(nativeOutput));
+      }
+      catch (Exception e)
+      {
+        return Wrappers_Compile.Result<software.amazon.cryptography.keystore.internaldafny.types._IWriteNewEncryptedBranchKeyVersionOutput, software.amazon.cryptography.keystore.internaldafny.types._IError>.create_Failure(TypeConversion.ToDafny_CommonError(e));
+      }
+    }
+    public Wrappers_Compile._IResult<software.amazon.cryptography.keystore.internaldafny.types._IWriteNewEncryptedBranchKeyVersionOutput, software.amazon.cryptography.keystore.internaldafny.types._IError> WriteNewEncryptedBranchKeyVersion_k(software.amazon.cryptography.keystore.internaldafny.types._IWriteNewEncryptedBranchKeyVersionInput input)
+    {
+      throw new KeyStoreException("Not supported at this time.");
+    }
+    public Wrappers_Compile._IResult<software.amazon.cryptography.keystore.internaldafny.types._IGetMutationLockAndIndexOutput, software.amazon.cryptography.keystore.internaldafny.types._IError> GetMutationLockAndIndex(software.amazon.cryptography.keystore.internaldafny.types._IGetMutationLockAndIndexInput input)
+    {
+      void validateOutput(AWS.Cryptography.KeyStore.GetMutationLockAndIndexOutput nativeOutput)
+      {
+        try { nativeOutput.Validate(); }
+        catch (ArgumentException e)
+        {
+          var message = $"Output of {_impl}._GetMutationLockAndIndex is invalid. {e.Message}";
+          throw new KeyStoreException(message);
+        }
+      }
+      AWS.Cryptography.KeyStore.GetMutationLockAndIndexInput nativeInput = TypeConversion.FromDafny_N3_aws__N12_cryptography__N8_keyStore__S28_GetMutationLockAndIndexInput(input);
+      try
+      {
+        AWS.Cryptography.KeyStore.GetMutationLockAndIndexOutput nativeOutput = _impl.GetMutationLockAndIndex(nativeInput);
+        _ = nativeOutput ?? throw new KeyStoreException($"{_impl}._GetMutationLockAndIndex returned null, should be {typeof(AWS.Cryptography.KeyStore.GetMutationLockAndIndexOutput)}");
+        validateOutput(nativeOutput);
+        return Wrappers_Compile.Result<software.amazon.cryptography.keystore.internaldafny.types._IGetMutationLockAndIndexOutput, software.amazon.cryptography.keystore.internaldafny.types._IError>.create_Success(TypeConversion.ToDafny_N3_aws__N12_cryptography__N8_keyStore__S29_GetMutationLockAndIndexOutput(nativeOutput));
+      }
+      catch (Exception e)
+      {
+        return Wrappers_Compile.Result<software.amazon.cryptography.keystore.internaldafny.types._IGetMutationLockAndIndexOutput, software.amazon.cryptography.keystore.internaldafny.types._IError>.create_Failure(TypeConversion.ToDafny_CommonError(e));
+      }
+    }
+    public Wrappers_Compile._IResult<software.amazon.cryptography.keystore.internaldafny.types._IGetMutationLockAndIndexOutput, software.amazon.cryptography.keystore.internaldafny.types._IError> GetMutationLockAndIndex_k(software.amazon.cryptography.keystore.internaldafny.types._IGetMutationLockAndIndexInput input)
+    {
+      throw new KeyStoreException("Not supported at this time.");
+    }
+    public Wrappers_Compile._IResult<software.amazon.cryptography.keystore.internaldafny.types._IQueryForVersionsOutput, software.amazon.cryptography.keystore.internaldafny.types._IError> QueryForVersions(software.amazon.cryptography.keystore.internaldafny.types._IQueryForVersionsInput input)
+    {
+      void validateOutput(AWS.Cryptography.KeyStore.QueryForVersionsOutput nativeOutput)
+      {
+        try { nativeOutput.Validate(); }
+        catch (ArgumentException e)
+        {
+          var message = $"Output of {_impl}._QueryForVersions is invalid. {e.Message}";
+          throw new KeyStoreException(message);
+        }
+      }
+      AWS.Cryptography.KeyStore.QueryForVersionsInput nativeInput = TypeConversion.FromDafny_N3_aws__N12_cryptography__N8_keyStore__S21_QueryForVersionsInput(input);
+      try
+      {
+        AWS.Cryptography.KeyStore.QueryForVersionsOutput nativeOutput = _impl.QueryForVersions(nativeInput);
+        _ = nativeOutput ?? throw new KeyStoreException($"{_impl}._QueryForVersions returned null, should be {typeof(AWS.Cryptography.KeyStore.QueryForVersionsOutput)}");
+        validateOutput(nativeOutput);
+        return Wrappers_Compile.Result<software.amazon.cryptography.keystore.internaldafny.types._IQueryForVersionsOutput, software.amazon.cryptography.keystore.internaldafny.types._IError>.create_Success(TypeConversion.ToDafny_N3_aws__N12_cryptography__N8_keyStore__S22_QueryForVersionsOutput(nativeOutput));
+      }
+      catch (Exception e)
+      {
+        return Wrappers_Compile.Result<software.amazon.cryptography.keystore.internaldafny.types._IQueryForVersionsOutput, software.amazon.cryptography.keystore.internaldafny.types._IError>.create_Failure(TypeConversion.ToDafny_CommonError(e));
+      }
+    }
+    public Wrappers_Compile._IResult<software.amazon.cryptography.keystore.internaldafny.types._IQueryForVersionsOutput, software.amazon.cryptography.keystore.internaldafny.types._IError> QueryForVersions_k(software.amazon.cryptography.keystore.internaldafny.types._IQueryForVersionsInput input)
+    {
+      throw new KeyStoreException("Not supported at this time.");
+    }
+    public Wrappers_Compile._IResult<software.amazon.cryptography.keystore.internaldafny.types._IUpdateMutationIndexOutput, software.amazon.cryptography.keystore.internaldafny.types._IError> UpdateMutationIndex(software.amazon.cryptography.keystore.internaldafny.types._IUpdateMutationIndexInput input)
+    {
+      void validateOutput(AWS.Cryptography.KeyStore.UpdateMutationIndexOutput nativeOutput)
+      {
+        try { nativeOutput.Validate(); }
+        catch (ArgumentException e)
+        {
+          var message = $"Output of {_impl}._UpdateMutationIndex is invalid. {e.Message}";
+          throw new KeyStoreException(message);
+        }
+      }
+      AWS.Cryptography.KeyStore.UpdateMutationIndexInput nativeInput = TypeConversion.FromDafny_N3_aws__N12_cryptography__N8_keyStore__S24_UpdateMutationIndexInput(input);
+      try
+      {
+        AWS.Cryptography.KeyStore.UpdateMutationIndexOutput nativeOutput = _impl.UpdateMutationIndex(nativeInput);
+        _ = nativeOutput ?? throw new KeyStoreException($"{_impl}._UpdateMutationIndex returned null, should be {typeof(AWS.Cryptography.KeyStore.UpdateMutationIndexOutput)}");
+        validateOutput(nativeOutput);
+        return Wrappers_Compile.Result<software.amazon.cryptography.keystore.internaldafny.types._IUpdateMutationIndexOutput, software.amazon.cryptography.keystore.internaldafny.types._IError>.create_Success(TypeConversion.ToDafny_N3_aws__N12_cryptography__N8_keyStore__S25_UpdateMutationIndexOutput(nativeOutput));
+      }
+      catch (Exception e)
+      {
+        return Wrappers_Compile.Result<software.amazon.cryptography.keystore.internaldafny.types._IUpdateMutationIndexOutput, software.amazon.cryptography.keystore.internaldafny.types._IError>.create_Failure(TypeConversion.ToDafny_CommonError(e));
+      }
+    }
+    public Wrappers_Compile._IResult<software.amazon.cryptography.keystore.internaldafny.types._IUpdateMutationIndexOutput, software.amazon.cryptography.keystore.internaldafny.types._IError> UpdateMutationIndex_k(software.amazon.cryptography.keystore.internaldafny.types._IUpdateMutationIndexInput input)
     {
       throw new KeyStoreException("Not supported at this time.");
     }
