AwsCryptographicMaterialProviders/runtimes/net/Generated/AwsCryptographyKeyStore/UpdateMutationIndexOutput.cs
@@ -5,7 +5,7 @@ using System;
 using AWS.Cryptography.KeyStore;
 namespace AWS.Cryptography.KeyStore
 {
-  public class DeleteMutationOutput
+  public class UpdateMutationIndexOutput
   {
 
 
