AwsCryptographicMaterialProviders/runtimes/python/src/aws_cryptographic_material_providers/smithygenerated/aws_cryptography_keystore/references.py
@@ -17,10 +17,14 @@ from aws_cryptographic_material_providers.internaldafny.generated.AwsCryptograph
     GetItemsForInitializeMutationOutput_GetItemsForInitializeMutationOutput as DafnyGetItemsForInitializeMutationOutput,
     GetKeyStorageInfoInput_GetKeyStorageInfoInput as DafnyGetKeyStorageInfoInput,
     GetKeyStorageInfoOutput_GetKeyStorageInfoOutput as DafnyGetKeyStorageInfoOutput,
-    GetMutationInput_GetMutationInput as DafnyGetMutationInput,
-    GetMutationOutput_GetMutationOutput as DafnyGetMutationOutput,
+    GetMutationLockAndIndexInput_GetMutationLockAndIndexInput as DafnyGetMutationLockAndIndexInput,
+    GetMutationLockAndIndexOutput_GetMutationLockAndIndexOutput as DafnyGetMutationLockAndIndexOutput,
+    GetMutationLockInput_GetMutationLockInput as DafnyGetMutationLockInput,
+    GetMutationLockOutput_GetMutationLockOutput as DafnyGetMutationLockOutput,
     QueryForVersionsInput_QueryForVersionsInput as DafnyQueryForVersionsInput,
     QueryForVersionsOutput_QueryForVersionsOutput as DafnyQueryForVersionsOutput,
+    UpdateMutationIndexInput_UpdateMutationIndexInput as DafnyUpdateMutationIndexInput,
+    UpdateMutationIndexOutput_UpdateMutationIndexOutput as DafnyUpdateMutationIndexOutput,
     WriteInitializeMutationInput_WriteInitializeMutationInput as DafnyWriteInitializeMutationInput,
     WriteInitializeMutationOutput_WriteInitializeMutationOutput as DafnyWriteInitializeMutationOutput,
     WriteMutatedVersionsInput_WriteMutatedVersionsInput as DafnyWriteMutatedVersionsInput,
@@ -66,10 +70,14 @@ class IKeyStorageInterface(metaclass=abc.ABCMeta):
             and callable(subclass.QueryForVersions)
             and hasattr(subclass, "WriteMutatedVersions")
             and callable(subclass.WriteMutatedVersions)
-            and hasattr(subclass, "GetMutation")
-            and callable(subclass.GetMutation)
-            and hasattr(subclass, "DeleteMutation")
-            and callable(subclass.DeleteMutation)
+            and hasattr(subclass, "UpdateMutationIndex")
+            and callable(subclass.UpdateMutationIndex)
+            and hasattr(subclass, "GetMutationLock")
+            and callable(subclass.GetMutationLock)
+            and hasattr(subclass, "GetMutationLockAndIndex")
+            and callable(subclass.GetMutationLockAndIndex)
+            and hasattr(subclass, "DeleteMutationLockAndIndex")
+            and callable(subclass.DeleteMutationLockAndIndex)
         )
 
     @abc.abstractmethod
@@ -162,7 +170,7 @@ class IKeyStorageInterface(metaclass=abc.ABCMeta):
         param: "aws_cryptographic_material_providers.smithygenerated.aws_cryptography_keystore.models.GetItemsForInitializeMutationInput",
     ) -> "aws_cryptographic_material_providers.smithygenerated.aws_cryptography_keystore.models.GetItemsForInitializeMutationOutput":
         """Gets the ACTIVE branch key and the beacon key, and looks for a
-        Mutation Commitment & Index, returning them if found."""
+        Mutation Lock & Index, returning them if found."""
         raise NotImplementedError
 
     @abc.abstractmethod
@@ -177,9 +185,8 @@ class IKeyStorageInterface(metaclass=abc.ABCMeta):
         -
         version (decrypt only) for new ACTIVE
         - beacon key
-        - mutated Versions
-        Also
-        writes the Mutation Commitment & Index.
+        Also writes the Mutation
+        Lock & Index.
         """
         raise NotImplementedError
 
@@ -204,12 +211,15 @@ class IKeyStorageInterface(metaclass=abc.ABCMeta):
         - every version already exsisting
         - every
         version's enc has not changed
-        - the Mutation Commitment has not changed
+        - the original of a Mutation Lock commits to the
+        original provided
+        - the terminal of a Mutation Lock commits to the terminal
+        provided
         """
         raise NotImplementedError
 
     @abc.abstractmethod
-    def get_mutation(
+    def update_mutation_index(
         self,
         param: "aws_cryptographic_materialproviders.smithygenerated.aws_cryptography_keystore.models.UpdateMutationIndexInput",
     ) -> "aws_cryptographic_materialproviders.smithygenerated.aws_cryptography_keystore.models.UpdateMutationIndexOutput":
@@ -229,7 +239,7 @@ class IKeyStorageInterface(metaclass=abc.ABCMeta):
         raise NotImplementedError
 
     @abc.abstractmethod
-    def delete_mutation(
+    def get_mutation_lock_and_index(
         self,
         param: "aws_cryptographic_material_providers.smithygenerated.aws_cryptography_keystore.models.ClobberMutationLockInput",
     ) -> "aws_cryptographic_material_providers.smithygenerated.aws_cryptography_keystore.models.ClobberMutationLockOutput":
@@ -446,20 +456,20 @@ class IKeyStorageInterface(metaclass=abc.ABCMeta):
             error = _smithy_error_to_dafny_error(e)
             return Wrappers.Result_Failure(error)
 
-    def GetMutation(
-        self, dafny_input: "DafnyGetMutationInput"
-    ) -> "DafnyGetMutationOutput":
+    def UpdateMutationIndex(
+        self, dafny_input: "DafnyUpdateMutationIndexInput"
+    ) -> "DafnyUpdateMutationIndexOutput":
         """Do not use.
 
         This method allows custom implementations of this interface to
         interact with generated code.
         """
-        native_input = aws_cryptographic_materialproviders.smithygenerated.aws_cryptography_keystore.dafny_to_smithy.aws_cryptography_keystore_GetMutationInput(
+        native_input = aws_cryptographic_materialproviders.smithygenerated.aws_cryptography_keystore.dafny_to_smithy.aws_cryptography_keystore_UpdateMutationIndexInput(
             dafny_input
         )
         try:
-            native_output = self.get_mutation(native_input)
-            dafny_output = aws_cryptographic_materialproviders.smithygenerated.aws_cryptography_keystore.smithy_to_dafny.aws_cryptography_keystore_GetMutationOutput(
+            native_output = self.update_mutation_index(native_input)
+            dafny_output = aws_cryptographic_materialproviders.smithygenerated.aws_cryptography_keystore.smithy_to_dafny.aws_cryptography_keystore_UpdateMutationIndexOutput(
                 native_output
             )
             return Wrappers.Result_Success(dafny_output)
@@ -467,9 +477,9 @@ class IKeyStorageInterface(metaclass=abc.ABCMeta):
             error = _smithy_error_to_dafny_error(e)
             return Wrappers.Result_Failure(error)
 
-    def DeleteMutation(
-        self, dafny_input: "DafnyDeleteMutationInput"
-    ) -> "DafnyDeleteMutationOutput":
+    def GetMutationLock(
+        self, dafny_input: "DafnyGetMutationLockInput"
+    ) -> "DafnyGetMutationLockOutput":
         """Do not use.
 
         This method allows custom implementations of this interface to
@@ -695,7 +705,7 @@ class KeyStorageInterface(IKeyStorageInterface):
         param: "aws_cryptographic_material_providers.smithygenerated.aws_cryptography_keystore.models.GetItemsForInitializeMutationInput",
     ) -> "aws_cryptographic_material_providers.smithygenerated.aws_cryptography_keystore.models.GetItemsForInitializeMutationOutput":
         """Gets the ACTIVE branch key and the beacon key, and looks for a
-        Mutation Commitment & Index, returning them if found."""
+        Mutation Lock & Index, returning them if found."""
         dafny_output = self._impl.GetItemsForInitializeMutation(
             aws_cryptographic_material_providers.smithygenerated.aws_cryptography_keystore.smithy_to_dafny.aws_cryptography_keystore_GetItemsForInitializeMutationInput(
                 param
@@ -724,9 +734,8 @@ class KeyStorageInterface(IKeyStorageInterface):
         -
         version (decrypt only) for new ACTIVE
         - beacon key
-        - mutated Versions
-        Also
-        writes the Mutation Commitment & Index.
+        Also writes the Mutation
+        Lock & Index.
         """
         dafny_output = self._impl.WriteInitializeMutation(
             aws_cryptographic_material_providers.smithygenerated.aws_cryptography_keystore.smithy_to_dafny.aws_cryptography_keystore_WriteInitializeMutationInput(
@@ -779,7 +788,10 @@ class KeyStorageInterface(IKeyStorageInterface):
         - every version already exsisting
         - every
         version's enc has not changed
-        - the Mutation Commitment has not changed
+        - the original of a Mutation Lock commits to the
+        original provided
+        - the terminal of a Mutation Lock commits to the terminal
+        provided
         """
         dafny_output = self._impl.WriteMutatedVersions(
             aws_cryptographic_material_providers.smithygenerated.aws_cryptography_keystore.smithy_to_dafny.aws_cryptography_keystore_WriteMutatedVersionsInput(
@@ -798,7 +810,7 @@ class KeyStorageInterface(IKeyStorageInterface):
                 dafny_output.value
             )
 
-    def get_mutation(
+    def update_mutation_index(
         self,
         param: "aws_cryptographic_materialproviders.smithygenerated.aws_cryptography_keystore.models.UpdateMutationIndexInput",
     ) -> "aws_cryptographic_materialproviders.smithygenerated.aws_cryptography_keystore.models.UpdateMutationIndexOutput":
@@ -846,7 +858,7 @@ class KeyStorageInterface(IKeyStorageInterface):
                 dafny_output.value
             )
 
-    def delete_mutation(
+    def get_mutation_lock_and_index(
         self,
         param: "aws_cryptographic_material_providers.smithygenerated.aws_cryptography_keystore.models.ClobberMutationLockInput",
     ) -> "aws_cryptographic_material_providers.smithygenerated.aws_cryptography_keystore.models.ClobberMutationLockOutput":
