AwsCryptographicMaterialProviders/runtimes/python/src/aws_cryptographic_material_providers/smithygenerated/aws_cryptography_keystore/smithy_to_dafny.py
@@ -13,8 +13,8 @@ from aws_cryptographic_material_providers.internaldafny.generated.AwsCryptograph
     CreateKeyOutput_CreateKeyOutput as DafnyCreateKeyOutput,
     CreateKeyStoreInput_CreateKeyStoreInput as DafnyCreateKeyStoreInput,
     CreateKeyStoreOutput_CreateKeyStoreOutput as DafnyCreateKeyStoreOutput,
-    DeleteMutationInput_DeleteMutationInput as DafnyDeleteMutationInput,
-    DeleteMutationOutput_DeleteMutationOutput as DafnyDeleteMutationOutput,
+    DeleteMutationLockAndIndexInput_DeleteMutationLockAndIndexInput as DafnyDeleteMutationLockAndIndexInput,
+    DeleteMutationLockAndIndexOutput_DeleteMutationLockAndIndexOutput as DafnyDeleteMutationLockAndIndexOutput,
     Discovery_Discovery as DafnyDiscovery,
     DynamoDBTable_DynamoDBTable as DafnyDynamoDBTable,
     EncryptedHierarchicalKey_EncryptedHierarchicalKey as DafnyEncryptedHierarchicalKey,
@@ -35,8 +35,10 @@ from aws_cryptographic_material_providers.internaldafny.generated.AwsCryptograph
     GetKeyStorageInfoInput_GetKeyStorageInfoInput as DafnyGetKeyStorageInfoInput,
     GetKeyStorageInfoOutput_GetKeyStorageInfoOutput as DafnyGetKeyStorageInfoOutput,
     GetKeyStoreInfoOutput_GetKeyStoreInfoOutput as DafnyGetKeyStoreInfoOutput,
-    GetMutationInput_GetMutationInput as DafnyGetMutationInput,
-    GetMutationOutput_GetMutationOutput as DafnyGetMutationOutput,
+    GetMutationLockAndIndexInput_GetMutationLockAndIndexInput as DafnyGetMutationLockAndIndexInput,
+    GetMutationLockAndIndexOutput_GetMutationLockAndIndexOutput as DafnyGetMutationLockAndIndexOutput,
+    GetMutationLockInput_GetMutationLockInput as DafnyGetMutationLockInput,
+    GetMutationLockOutput_GetMutationLockOutput as DafnyGetMutationLockOutput,
     HierarchicalKeyType_ActiveHierarchicalSymmetricBeacon,
     HierarchicalKeyType_ActiveHierarchicalSymmetricVersion,
     HierarchicalKeyType_HierarchicalSymmetricVersion,
@@ -48,14 +50,15 @@ from aws_cryptographic_material_providers.internaldafny.generated.AwsCryptograph
     KeyManagement_kms,
     KeyStoreConfig_KeyStoreConfig as DafnyKeyStoreConfig,
     MRDiscovery_MRDiscovery as DafnyMRDiscovery,
-    MutationCommitment_MutationCommitment as DafnyMutationCommitment,
     MutationIndex_MutationIndex as DafnyMutationIndex,
+    MutationLock_MutationLock as DafnyMutationLock,
     OverWriteEncryptedHierarchicalKey_OverWriteEncryptedHierarchicalKey as DafnyOverWriteEncryptedHierarchicalKey,
-    OverWriteMutationIndex_OverWriteMutationIndex as DafnyOverWriteMutationIndex,
     QueryForVersionsInput_QueryForVersionsInput as DafnyQueryForVersionsInput,
     QueryForVersionsOutput_QueryForVersionsOutput as DafnyQueryForVersionsOutput,
     Storage_custom,
     Storage_ddb,
+    UpdateMutationIndexInput_UpdateMutationIndexInput as DafnyUpdateMutationIndexInput,
+    UpdateMutationIndexOutput_UpdateMutationIndexOutput as DafnyUpdateMutationIndexOutput,
     VersionKeyInput_VersionKeyInput as DafnyVersionKeyInput,
     VersionKeyOutput_VersionKeyOutput as DafnyVersionKeyOutput,
     WriteInitializeMutationInput_WriteInitializeMutationInput as DafnyWriteInitializeMutationInput,
@@ -362,7 +365,7 @@ def aws_cryptography_keystore_GetItemsForInitializeMutationOutput(native_input):
         BeaconItem=aws_cryptographic_material_providers.smithygenerated.aws_cryptography_keystore.smithy_to_dafny.aws_cryptography_keystore_EncryptedHierarchicalKey(
             native_input.beacon_item
         ),
-        MutationCommitment=(
+        MutationLock=(
             (
                 Option_Some(
                     aws_cryptographic_material_providers.smithygenerated.aws_cryptography_keystore.smithy_to_dafny.aws_cryptography_keystore_MutationLock(
@@ -370,7 +373,7 @@ def aws_cryptography_keystore_GetItemsForInitializeMutationOutput(native_input):
                     )
                 )
             )
-            if (native_input.mutation_commitment is not None)
+            if (native_input.mutation_lock is not None)
             else (Option_None())
         ),
         MutationIndex=(
@@ -387,8 +390,8 @@ def aws_cryptography_keystore_GetItemsForInitializeMutationOutput(native_input):
     )
 
 
-def aws_cryptography_keystore_MutationCommitment(native_input):
-    return DafnyMutationCommitment(
+def aws_cryptography_keystore_MutationLock(native_input):
+    return DafnyMutationLock(
         Identifier=Seq(
             "".join(
                 [
@@ -419,7 +422,6 @@ def aws_cryptography_keystore_MutationCommitment(native_input):
         ),
         Original=Seq(native_input.original),
         Terminal=Seq(native_input.terminal),
-        Input=Seq(native_input.input),
         CiphertextBlob=Seq(native_input.ciphertext_blob),
     )
 
@@ -569,13 +571,9 @@ def aws_cryptography_keystore_WriteMutatedVersionsInput(native_input):
                 for list_element in native_input.items
             ]
         ),
-        MutationCommitment=aws_cryptographic_materialproviders.smithygenerated.aws_cryptography_keystore.smithy_to_dafny.aws_cryptography_keystore_MutationCommitment(
-            native_input.mutation_commitment
+        MutationLock=aws_cryptographic_materialproviders.smithygenerated.aws_cryptography_keystore.smithy_to_dafny.aws_cryptography_keystore_MutationLock(
+            native_input.mutation_lock
         ),
-        MutationIndex=aws_cryptographic_materialproviders.smithygenerated.aws_cryptography_keystore.smithy_to_dafny.aws_cryptography_keystore_OverWriteMutationIndex(
-            native_input.mutation_index
-        ),
-        EndMutation=native_input.end_mutation,
     )
 
 
@@ -583,8 +581,23 @@ def aws_cryptography_keystore_WriteMutatedVersionsOutput(native_input):
     return DafnyWriteMutatedVersionsOutput()
 
 
-def aws_cryptography_keystore_GetMutationInput(native_input):
-    return DafnyGetMutationInput(
+def aws_cryptography_keystore_UpdateMutationIndexInput(native_input):
+    return DafnyUpdateMutationIndexInput(
+        MutationIndex=aws_cryptographic_materialproviders.smithygenerated.aws_cryptography_keystore.smithy_to_dafny.aws_cryptography_keystore_MutationIndex(
+            native_input.mutation_index
+        ),
+        OldMutationIndex=aws_cryptographic_materialproviders.smithygenerated.aws_cryptography_keystore.smithy_to_dafny.aws_cryptography_keystore_MutationIndex(
+            native_input.old_mutation_index
+        ),
+    )
+
+
+def aws_cryptography_keystore_UpdateMutationIndexOutput(native_input):
+    return DafnyUpdateMutationIndexOutput()
+
+
+def aws_cryptography_keystore_GetMutationLockInput(native_input):
+    return DafnyGetMutationLockInput(
         Identifier=Seq(
             "".join(
                 [
@@ -598,9 +611,9 @@ def aws_cryptography_keystore_GetMutationInput(native_input):
     )
 
 
-def aws_cryptography_keystore_GetMutationOutput(native_input):
-    return DafnyGetMutationOutput(
-        MutationCommitment=(
+def aws_cryptography_keystore_GetMutationLockOutput(native_input):
+    return DafnyGetMutationLockOutput(
+        MutationLock=(
             (
                 Option_Some(
                     aws_cryptographic_material_providers.smithygenerated.aws_cryptography_keystore.smithy_to_dafny.aws_cryptography_keystore_MutationLock(
@@ -622,8 +635,8 @@ def aws_cryptography_keystore_ClobberMutationLockInput(native_input):
     )
 
 
-def aws_cryptography_keystore_DeleteMutationOutput(native_input):
-    return DafnyDeleteMutationOutput()
+def aws_cryptography_keystore_DeleteMutationLockAndIndexOutput(native_input):
+    return DafnyDeleteMutationLockAndIndexOutput()
 
 
 def smithy_api_Unit(native_input):
